Wibbles around module names

coq/MMap.v
@@ -5,8 +5,9 @@ Require SetoidClass. (* (==) from SetoidClass clashes with stuff from MMaps. Ugh
 Module SC := SetoidClass.
 
 Module VMMap (X : OrderedType) (D : OrderedType) (Import P: OrderedLattice D).
-  Module M      := Make_ord X D.
-  Module MProps := WProperties_fun X M.MapS.
+  Module M'     := Make_ord X D.
+  Module M      := M'.MapS.
+  Module MProps := WProperties_fun X M.
 
   (* Useful tactics *)
 
@@ -15,8 +16,8 @@ Module VMMap (X : OrderedType) (D : OrderedType) (Import P: OrderedLattice D).
   (* Some useful auxiliary definitions *)
 
   Definition raw_adjusti (f : X.t -> D.t -> D.t) (k : X.t)
-      : M.MapS.Raw.t D.t -> M.MapS.Raw.t D.t :=
-    fix go (m : M.MapS.Raw.t D.t) : M.MapS.Raw.t D.t :=
+      : M.Raw.t D.t -> M.Raw.t D.t :=
+    fix go (m : M.Raw.t D.t) : M.Raw.t D.t :=
       match m with
       | nil => nil
       | (kx, x) :: xs =>
@@ -27,25 +28,25 @@ Module VMMap (X : OrderedType) (D : OrderedType) (Import P: OrderedLattice D).
       end.
 
   Definition raw_adjust (f : D.t -> D.t)
-      : X.t -> M.MapS.Raw.t D.t -> M.MapS.Raw.t D.t :=
+      : X.t -> M.Raw.t D.t -> M.Raw.t D.t :=
     raw_adjusti (fun _ x => f x).
 
   Lemma adjusti_HdRel :
-    forall (f : X.t -> D.t -> D.t) (k1 k2 : X.t) (v : D.t) (m : M.MapS.Raw.t D.t),
-    HdRel M.MapS.Raw.PX.ltk (k1, v) m -> HdRel M.MapS.Raw.PX.ltk (k1, v) (raw_adjusti f k2 m).
+    forall (f : X.t -> D.t -> D.t) (k1 k2 : X.t) (v : D.t) (m : M.Raw.t D.t),
+    HdRel M.Raw.PX.ltk (k1, v) m -> HdRel M.Raw.PX.ltk (k1, v) (raw_adjusti f k2 m).
   Proof.
     intros. induction H; simpl; auto.
     destruct b. cdestruct (X.compare k2 t); auto.
   Qed.
 
   Lemma HdRel_ltk_value_unimportant :
-    forall {k : X.t} {v1 v2 : D.t} {m : M.MapS.Raw.t D.t},
-    HdRel M.MapS.Raw.PX.ltk (k, v1) m -> HdRel M.MapS.Raw.PX.ltk (k, v2) m.
+    forall {k : X.t} {v1 v2 : D.t} {m : M.Raw.t D.t},
+    HdRel M.Raw.PX.ltk (k, v1) m -> HdRel M.Raw.PX.ltk (k, v2) m.
   Proof. intros. destruct H; auto. Qed.
 
   Lemma adjusti_Sorted :
-    forall (f : X.t -> D.t -> D.t) (k : X.t) (m : M.MapS.Raw.t D.t),
-    Sorted M.MapS.Raw.PX.ltk m -> Sorted M.MapS.Raw.PX.ltk (raw_adjusti f k m).
+    forall (f : X.t -> D.t -> D.t) (k : X.t) (m : M.Raw.t D.t),
+    Sorted M.Raw.PX.ltk m -> Sorted M.Raw.PX.ltk (raw_adjusti f k m).
   Proof.
     intros. induction H; simpl; auto. destruct a.
     cdestruct (X.compare k t); constructor; try (apply adjusti_HdRel); auto.
@@ -53,38 +54,38 @@ Module VMMap (X : OrderedType) (D : OrderedType) (Import P: OrderedLattice D).
   Qed.
 
   Lemma adjust_Sorted :
-    forall (f : D.t -> D.t) (k : X.t) (m : M.MapS.Raw.t D.t),
-    Sorted M.MapS.Raw.PX.ltk m -> Sorted M.MapS.Raw.PX.ltk (raw_adjust f k m).
+    forall (f : D.t -> D.t) (k : X.t) (m : M.Raw.t D.t),
+    Sorted M.Raw.PX.ltk m -> Sorted M.Raw.PX.ltk (raw_adjust f k m).
   Proof. intros. apply adjusti_Sorted. auto. Qed.
 
-  Definition adjusti (f : X.t -> D.t -> D.t) (k : X.t) (m : M.MapS.t D.t) : M.MapS.t D.t :=
-    M.MapS.Mk (adjusti_Sorted f k m.(M.MapS.this) m.(M.MapS.sorted)).
+  Definition adjusti (f : X.t -> D.t -> D.t) (k : X.t) (m : M.t D.t) : M.t D.t :=
+    M.Mk (adjusti_Sorted f k m.(M.this) m.(M.sorted)).
 
-  Definition adjust (f : D.t -> D.t) (k : X.t) (m : M.MapS.t D.t) : M.MapS.t D.t :=
-    M.MapS.Mk (adjust_Sorted f k m.(M.MapS.this) m.(M.MapS.sorted)).
+  Definition adjust (f : D.t -> D.t) (k : X.t) (m : M.t D.t) : M.t D.t :=
+    M.Mk (adjust_Sorted f k m.(M.this) m.(M.sorted)).
 
   (* Proofs and stuff *)
 
-  Instance eq_list_refl : Reflexive M.eq_list := {}.
+  Instance eq_list_refl : Reflexive M'.eq_list := {}.
   Proof.
     induction x.
     - reflexivity.
-    - simpl. destruct a. rewrite M.MapS.Raw.MX.compare_refl. split.
+    - simpl. destruct a. rewrite M.Raw.MX.compare_refl. split.
       + reflexivity.
       + auto.
   Qed.
-  Instance eq_list_sym : Symmetric M.eq_list := {}.
+  Instance eq_list_sym : Symmetric M'.eq_list := {}.
   Proof.
     induction x; induction y; simpl; try contradiction; auto.
     - destruct a. contradiction.
     - destruct a, a0. cdestruct (X.compare t t1); try contradiction.
       assert (Hsym := H). symmetry in Hsym.
-      rewrite (iff_sym (M.MapS.Raw.MX.compare_eq_iff t1 t)) in Hsym. rewrite Hsym.
+      rewrite (iff_sym (M.Raw.MX.compare_eq_iff t1 t)) in Hsym. rewrite Hsym.
       intro. destruct H0. split.
       + symmetry. auto.
       + auto.
   Qed.
-  Instance eq_list_trans : Transitive M.eq_list := {}.
+  Instance eq_list_trans : Transitive M'.eq_list := {}.
   Proof.
     induction x; induction y; induction z; simpl; try contradiction; auto.
     - destruct a0. contradiction.
@@ -92,15 +93,15 @@ Module VMMap (X : OrderedType) (D : OrderedType) (Import P: OrderedLattice D).
       cdestruct (X.compare t t1); try contradiction.
       cdestruct (X.compare t1 t3); try contradiction.
       assert (tEqT3 : X.eq t t3). { rewrite H. auto. }
-      rewrite (iff_sym (M.MapS.Raw.MX.compare_eq_iff t t3)) in tEqT3. rewrite tEqT3.
+      rewrite (iff_sym (M.Raw.MX.compare_eq_iff t t3)) in tEqT3. rewrite tEqT3.
       intros. destruct H1, H2. split.
       + rewrite H1. auto.
       + apply IHx with (y := y); auto.
   Qed.
-  Instance eq_list_equiv : Equivalence M.eq_list := {}.
+  Instance eq_list_equiv : Equivalence M'.eq_list := {}.
 
-  Instance Setoid : SC.Setoid (M.MapS.t D.t) := {
-    equiv := M.eq
+  Instance Setoid : SC.Setoid (M.t D.t) := {
+    equiv := M'.eq
   }.
 
   Definition union_f (key : X.t) (oe1 oe2 : option D.t) : option D.t :=
@@ -111,20 +112,20 @@ Module VMMap (X : OrderedType) (D : OrderedType) (Import P: OrderedLattice D).
     | Some e1, Some e2 => Some (join e1 e2)
     end.
 
-  Definition union : M.MapS.t D.t -> M.MapS.t D.t -> M.MapS.t D.t :=
-    M.MapS.merge union_f.
+  Definition union : M.t D.t -> M.t D.t -> M.t D.t :=
+    M.merge union_f.
 
-  Instance JSL : JoinSemiLattice (M.MapS.t D.t) := {
+  Instance JSL : JoinSemiLattice (M.t D.t) := {
     join := union
   }.
 
-  Instance BJSL : BoundedJoinSemiLattice (M.MapS.t D.t) := {
-    bottom := M.MapS.empty
+  Instance BJSL : BoundedJoinSemiLattice (M.t D.t) := {
+    bottom := M.empty
   }.
 
   Lemma merge_l_union_id :
-    forall (m : M.MapS.Raw.t D.t),
-    M.MapS.Raw.merge_l union_f m = m.
+    forall (m : M.Raw.t D.t),
+    M.Raw.merge_l union_f m = m.
   Proof.
     intros. induction m; simpl.
     - auto.
@@ -132,8 +133,8 @@ Module VMMap (X : OrderedType) (D : OrderedType) (Import P: OrderedLattice D).
   Qed.
 
   Lemma merge_r_union_id :
-    forall (m : M.MapS.Raw.t D.t),
-    M.MapS.Raw.merge_r union_f m = m.
+    forall (m : M.Raw.t D.t),
+    M.Raw.merge_r union_f m = m.
   Proof.
     intros. induction m; simpl.
     - auto.
@@ -141,35 +142,35 @@ Module VMMap (X : OrderedType) (D : OrderedType) (Import P: OrderedLattice D).
   Qed.
 
   Lemma merge_union_nil_r :
-    forall (m : M.MapS.Raw.t D.t),
-    M.eq_list (M.MapS.Raw.merge union_f m nil) m.
+    forall (m : M.Raw.t D.t),
+    M'.eq_list (M.Raw.merge union_f m nil) m.
   Proof.
     destruct m; simpl.
     - constructor.
-    - destruct p. simpl. rewrite M.MapS.Raw.MX.compare_refl. split.
+    - destruct p. simpl. rewrite M.Raw.MX.compare_refl. split.
       + reflexivity.
       + rewrite merge_l_union_id. reflexivity.
   Qed.
 
   Lemma eq_to_compare : forall a b, X.eq a b -> X.compare a b = Eq.
-  Proof. intros. rewrite (M.MapS.Raw.MX.compare_eq_iff a b). auto. Qed.
+  Proof. intros. rewrite (M.Raw.MX.compare_eq_iff a b). auto. Qed.
 
   Lemma lt_to_compare : forall a b, X.lt a b -> X.compare a b = Lt.
-  Proof. intros. rewrite (M.MapS.Raw.MX.compare_lt_iff a b). auto. Qed.
+  Proof. intros. rewrite (M.Raw.MX.compare_lt_iff a b). auto. Qed.
 
   Lemma gt_to_compare : forall a b, X.lt a b -> X.compare b a = Gt.
-  Proof. intros. rewrite (M.MapS.Raw.MX.compare_gt_iff b a). auto. Qed.
+  Proof. intros. rewrite (M.Raw.MX.compare_gt_iff b a). auto. Qed.
 
   Lemma merge_union_associative :
-    forall (m1 m2 m3 : M.MapS.Raw.t D.t),
-    M.eq_list (M.MapS.Raw.merge union_f m1 (M.MapS.Raw.merge union_f m2 m3))
-              (M.MapS.Raw.merge union_f (M.MapS.Raw.merge union_f m1 m2) m3).
+    forall (m1 m2 m3 : M.Raw.t D.t),
+    M'.eq_list (M.Raw.merge union_f m1 (M.Raw.merge union_f m2 m3))
+               (M.Raw.merge union_f (M.Raw.merge union_f m1 m2) m3).
   Proof.
     Ltac crush :=
     repeat match goal with
-    | |- context[M.MapS.Raw.merge_l union_f ?m] => rewrite (merge_l_union_id m); simpl
-    | |- context[M.MapS.Raw.merge_r union_f ?m] => rewrite (merge_r_union_id m); simpl
-    | |- context[M.MapS.Raw.merge union_f ?m nil] => rewrite (merge_union_nil_r m); simpl
+    | |- context[M.Raw.merge_l union_f ?m] => rewrite (merge_l_union_id m); simpl
+    | |- context[M.Raw.merge_r union_f ?m] => rewrite (merge_r_union_id m); simpl
+    | |- context[M.Raw.merge union_f ?m nil] => rewrite (merge_union_nil_r m); simpl
     | Heq : X.eq ?a ?b |- context[X.compare ?a ?b] => rewrite (eq_to_compare a b Heq); simpl
     | Heq1 : X.eq ?a ?b, Heq2 : X.eq ?b ?c |- context[X.compare ?a ?c] =>
         rewrite (eq_to_compare a c (Equivalence_Transitive (A := X.t) a b c Heq1 Heq2)); simpl
@@ -181,13 +182,13 @@ Module VMMap (X : OrderedType) (D : OrderedType) (Import P: OrderedLattice D).
        rewrite <- Heq in Hlt; rewrite (lt_to_compare a1 b Hlt); simpl
     | Heq : X.eq ?a1 ?a2, Hlt : X.lt ?b ?a2 |- context[X.compare ?a1 ?b] =>
        rewrite <- Heq in Hlt; rewrite (gt_to_compare b a1 Hlt); simpl
-    | |- context[X.compare ?t ?t] => rewrite M.MapS.Raw.MX.compare_refl
+    | |- context[X.compare ?t ?t] => rewrite M.Raw.MX.compare_refl
     | Heq : X.eq ?a1 ?a2, Hlt : X.lt ?b ?a1 |- context[X.compare ?b ?a2] =>
        rewrite Heq in Hlt; rewrite (lt_to_compare b a2 Hlt); simpl
     | Hlt1 : X.lt ?a1 ?a2, Hlt2 : X.lt ?a2 ?a3 |- context[X.compare ?a1 ?a3] =>
-       rewrite (lt_to_compare a1 a3 (M.MapS.Raw.MX.lt_trans Hlt1 Hlt2)); simpl
+       rewrite (lt_to_compare a1 a3 (M.Raw.MX.lt_trans Hlt1 Hlt2)); simpl
     | Hlt1 : X.lt ?a1 ?a2, Hlt2 : X.lt ?a2 ?a3 |- context[X.compare ?a3 ?a1] =>
-       rewrite (gt_to_compare a1 a3 (M.MapS.Raw.MX.lt_trans Hlt1 Hlt2)); simpl
+       rewrite (gt_to_compare a1 a3 (M.Raw.MX.lt_trans Hlt1 Hlt2)); simpl
     | |- context[match ?p with | pair _ _ => _ end] => destruct p; simpl
     | |- _ /\ _ => split
     | |- _ => auto; try reflexivity
@@ -215,15 +216,15 @@ Module VMMap (X : OrderedType) (D : OrderedType) (Import P: OrderedLattice D).
     Qed.
 
   Lemma merge_union_commutative :
-    forall (m1 m2 : M.MapS.Raw.t D.t),
-    M.eq_list (M.MapS.Raw.merge union_f m1 m2) (M.MapS.Raw.merge union_f m2 m1).
+    forall (m1 m2 : M.Raw.t D.t),
+    M'.eq_list (M.Raw.merge union_f m1 m2) (M.Raw.merge union_f m2 m1).
   Proof.
     induction m1; simpl.
     - intros. rewrite merge_r_union_id. rewrite merge_union_nil_r. reflexivity.
     - induction m2; destruct a; simpl;
       repeat rewrite merge_l_union_id;
       repeat rewrite merge_r_union_id.
-      + rewrite M.MapS.Raw.MX.compare_refl. split; reflexivity.
+      + rewrite M.Raw.MX.compare_refl. split; reflexivity.
       + destruct a0. simpl. cdestruct (X.compare t t1).
         * assert (Hsym := H). symmetry in Hsym.
           rewrite (eq_to_compare t1 t Hsym). simpl.
@@ -232,30 +233,30 @@ Module VMMap (X : OrderedType) (D : OrderedType) (Import P: OrderedLattice D).
              rewrite dequiv_is_deq in Comm. auto.
           -- auto.
         * rewrite (gt_to_compare t t1 H). simpl.
-          rewrite M.MapS.Raw.MX.compare_refl. split.
+          rewrite M.Raw.MX.compare_refl. split.
           -- reflexivity.
           -- specialize (IHm1 ((t1, t2) :: m2)). simpl in IHm1.
              repeat rewrite merge_l_union_id in IHm1. auto.
         * rewrite (lt_to_compare t1 t H). simpl.
-          rewrite M.MapS.Raw.MX.compare_refl. split.
+          rewrite M.Raw.MX.compare_refl. split.
           -- reflexivity.
           -- repeat rewrite merge_l_union_id in IHm2. auto.
   Qed.
 
   Lemma merge_union_idempotent :
-    forall (m : M.MapS.Raw.t D.t),
-    M.eq_list (M.MapS.Raw.merge union_f m m) m.
+    forall (m : M.Raw.t D.t),
+    M'.eq_list (M.Raw.merge union_f m m) m.
   Proof.
     induction m; simpl.
     + constructor.
-    + destruct a. rewrite M.MapS.Raw.MX.compare_refl. simpl.
-      rewrite M.MapS.Raw.MX.compare_refl. split.
+    + destruct a. rewrite M.Raw.MX.compare_refl. simpl.
+      rewrite M.Raw.MX.compare_refl. split.
       * pose proof (jslIdempotency (a := D.t)) as Idem. specialize (Idem t0).
         rewrite dequiv_is_deq in Idem. auto.
       * auto.
   Qed.
 
-  Instance VJSL : VJoinSemiLattice (M.MapS.t D.t) := {}.
+  Instance VJSL : VJoinSemiLattice (M.t D.t) := {}.
   Proof.
   - destruct x, y, z. apply merge_union_associative.
   - destruct x, y. apply merge_union_commutative.
@@ -264,6 +265,6 @@ Module VMMap (X : OrderedType) (D : OrderedType) (Import P: OrderedLattice D).
 
   Instance VBJSL :
     forall `{VJoinSemiLattice D.t},
-    VBoundedJoinSemiLattice (M.MapS.t D.t) := {}.
+    VBoundedJoinSemiLattice (M.t D.t) := {}.
   Proof. destruct x. apply merge_union_nil_r. Qed.
 End VMMap.
