coq/State.v
@@ -7,15 +7,15 @@ Require Import QArith.
 Require Import Structures.Equalities Structures.Orders Structures.OrdersEx.
 
 Module Max_Nat_as_OT := PairOrderedType Max_as_OT Nat_as_OT.
-Module S  := MSets.MSetAVL.Make Max_Nat_as_OT.
-Module VS := VMSet Max_Nat_as_OT S.
-Module VM := VMMap Nat_as_OT Max_as_OT Max_as_OL.
-Module M  := VM.M.
+Module SetPairMaxNat  := MSets.MSetAVL.Make Max_Nat_as_OT.
+Module VSetPairMaxNat := VMSet Max_Nat_as_OT SetPairMaxNat.
+Module VMapNat2Max := VMMap Nat_as_OT Max_as_OT Max_as_OL.
+Module MapNat2Max  := VMapNat2Max.M.
 
 Definition Time := Max.
-Definition TimeMap := M.t.
+Definition TimeMap := VMapNat2Max.M'.t.
 Definition TID := nat.
-Definition Log := S.t.
+Definition Log := SetPairMaxNat.t.
 
 Inductive State : Type :=
 | MkState : TimeMap -> Log -> State.
@@ -23,7 +23,7 @@ Inductive State : Type :=
 Definition StateEq (s1 s2 : State) : Prop :=
   match s1, s2 with
   | MkState t1 l1, MkState t2 l2 =>
-    M.eq t1 t2 /\ S.Equal l1 l2
+    VMapNat2Max.M'.eq t1 t2 /\ SetPairMaxNat.Equal l1 l2
   end.
 
 Instance StateEqReflexive : Reflexive StateEq := {}.
@@ -60,19 +60,19 @@ Instance State_BJSL : BoundedJoinSemiLattice State := {
 Instance State_VJSL : VJoinSemiLattice State := {}.
 Proof.
 - destruct x, y, z. split.
-  + destruct VM.VJSL. apply jslAssociativity.
-  + destruct VS.VJSL. apply jslAssociativity.
+  + destruct VMapNat2Max.VJSL. apply jslAssociativity.
+  + destruct VSetPairMaxNat.VJSL. apply jslAssociativity.
 - destruct x, y. split.
-  + destruct VM.VJSL. apply jslCommutativity.
-  + destruct VS.VJSL. apply jslCommutativity.
+  + destruct VMapNat2Max.VJSL. apply jslCommutativity.
+  + destruct VSetPairMaxNat.VJSL. apply jslCommutativity.
 - destruct x. split.
-  + destruct VM.VJSL. apply jslIdempotency.
-  + destruct VS.VJSL. apply jslIdempotency.
+  + destruct VMapNat2Max.VJSL. apply jslIdempotency.
+  + destruct VSetPairMaxNat.VJSL. apply jslIdempotency.
 Qed.
 
 Instance State_VBJSL : VBoundedJoinSemiLattice State := {}.
 Proof.
   destruct x. split.
-  - destruct VM.VBJSL. apply bjslIdentity.
-  - destruct VS.VBJSL. apply bjslIdentity.
+  - destruct VMapNat2Max.VBJSL. apply bjslIdentity.
+  - destruct VSetPairMaxNat.VBJSL. apply bjslIdentity.
 Qed.
